Tealeaves/Classes/Kleisli/DecoratedShapelyFunctor.v
@@ -9,20 +9,20 @@ Import Functor.Notations.
 Import Subset.Notations.
 Import List.ListNotations.
 
-(** * CtxTolist operation *)
+(** * ToCtxlist operation *)
 (******************************************************************************)
-Class CtxTolist (E : Type) (F : Type -> Type) :=
-  ctx_tolist : forall A : Type, F A -> env E A.
+Class ToCtxlist (E : Type) (F : Type -> Type) :=
+  toctxlist : forall A : Type, F A -> env E A.
 
-#[global] Arguments ctx_tolist {E}%type_scope {F}%function_scope
-      {CtxTolist} {A}%type_scope _.
+#[global] Arguments toctxlist {E}%type_scope {F}%function_scope
+      {ToCtxlist} {A}%type_scope _.
 
 (*
 (** * Shapely functors are containers *)
 (******************************************************************************)
 #[export] Instance Elementsd_Tolistd (E : Type) (F : Type -> Type)
   `{Tolistd E F} : CtxElements E F :=
-  fun A => element_of ∘ tolistd.
+  fun A => tosubset ∘ tolistd.
 
 Theorem ind_iff_ind_list (E : Type) (F : Type -> Type)
   `{Tolistd E F} : forall (A : Type) (t : F A) (e : E) (a : A),
